Rename BUFFER_SIZE to LOG_SIZE and adjust size closer to Rust impl.

concurrency/node-replication/Constants.i.dfy
@@ -3,7 +3,7 @@ include "../../lib/Lang/NativeTypes.s.dfy"
 module Constants {
   import opened NativeTypes
 
-  const GC_FROM_HEAD: uint64 := 32 * 256;
+  const LOG_SIZE: uint64 := 1024 * 1024;
   const WARN_THRESHOLD: uint64 := 0x1000_0000; // 1 << 28
 
   // Fixed number of replicas (in reference impl, this is variable)
@@ -11,9 +11,8 @@ module Constants {
 
   // Should be configured to the exact number of threads for best performance
   const MAX_THREADS_PER_REPLICA: uint64 := 256;
-
   const MAX_PENDING_OPS: uint64 := 1
-  const BUFFER_SIZE: uint64 := MAX_THREADS_PER_REPLICA * MAX_PENDING_OPS;
+  const GC_FROM_HEAD: uint64 := MAX_PENDING_OPS * MAX_THREADS_PER_REPLICA;
 
   // number of reference counts should be equal to the number of expected threads
   function method RC_WIDTH_64() : uint64 { MAX_THREADS_PER_REPLICA }
